src/tls/PSK.fst
@@ -1,5 +1,5 @@
 (*--build-config
-options:--use_hints --fstar_home ../../../FStar --include ../../../FStar/ucontrib/Platform/fst/ --include ../../../FStar/ucontrib/CoreCrypto/fst/ --include ../../../FStar/examples/low-level/crypto/real --include ../../../FStar/examples/low-level/crypto/spartan --include ../../../FStar/examples/low-level/LowCProvider/fst --include ../../../FStar/examples/low-level/crypto --include ../../libs/ffi --include ../../../FStar/ulib/hyperstack --include ideal-flags;
+options:--fstar_home ../../../FStar --max_fuel 4 --initial_fuel 0 --max_ifuel 2 --initial_ifuel 1 --z3rlimit 20 --__temp_no_proj Handshake --__temp_no_proj Connection --use_hints --include ../../../FStar/ucontrib/CoreCrypto/fst/ --include ../../../FStar/ucontrib/Platform/fst/ --include ../../../hacl-star/secure_api/LowCProvider/fst --include ../../../kremlin/kremlib --include ../../../hacl-star/specs --include ../../../hacl-star/code/lib/kremlin --include ../../../hacl-star/code/bignum --include ../../../hacl-star/code/experimental/aesgcm --include ../../../hacl-star/code/poly1305 --include ../../../hacl-star/code/salsa-family --include ../../../hacl-star/secure_api/test --include ../../../hacl-star/secure_api/utils --include ../../../hacl-star/secure_api/vale --include ../../../hacl-star/secure_api/uf1cma --include ../../../hacl-star/secure_api/prf --include ../../../hacl-star/secure_api/aead --include ../../libs/ffi --include ../../../FStar/ulib/hyperstack --include ../../src/tls/ideal-flags;
 --*)
 module PSK
 
@@ -21,7 +21,7 @@ module HS = FStar.HyperStack
 // <from TLSConstants>
 
 // TODO: give more precise type
-// move elsewhere? 
+// move elsewhere?
 
 (** PSK Identity definition *)
 type pskIdentity = b:bytes{repr_bytes (length b) <= 2}
@@ -319,7 +319,7 @@ let verify_hash (i:pskid) (a:hash_alg) : ST bool
     else false
 
 
-(* 
+(*
 Provisional support for the PSK extension
 https://tlswg.github.io/tls13-spec/#rfc.section.4.2.10
 
@@ -327,17 +327,17 @@ The PSK table should include (at least for tickets)
 
   time_created: UInt32.t // the server's viewpoint
   time_accepted: UInt32.t // the client's viewpoint
-  mask: UInt32.t 
-  livetime: UInt32.t 
+  mask: UInt32.t
+  livetime: UInt32.t
 
 The authenticated property of the binder should includes
 
-  ClientHello[ nonce, ... pskid, obfuscated_ticket_age] /\ 
-  psk = lookup pskid 
-  ==> 
-  exists client. 
+  ClientHello[ nonce, ... pskid, obfuscated_ticket_age] /\
+  psk = lookup pskid
+  ==>
+  exists client.
     client.nonce = nonce /\
-    let age = client.time_connected - psk.time_created in 
+    let age = client.time_connected - psk.time_created in
     age <= psk.livetime /\
     obfuscated_ticket_age = encode_age age
 
@@ -345,12 +345,11 @@ Hence, the server authenticates age, and may filter 0RTT accordingly.
 
 *)
 
-type ticket_age = UInt32.t 
-type obfuscated_ticket_age = UInt32.t 
+type ticket_age = UInt32.t
+type obfuscated_ticket_age = UInt32.t
 let default_obfuscated_age = 0ul
 open FStar.UInt32
 let encode_age (t:ticket_age)  mask = t +%^ mask
 let decode_age (t:obfuscated_ticket_age) mask = t -%^ mask
 
 private let inverse_mask t mask: Lemma (decode_age (encode_age t mask) mask = t) = ()
-
